% -*- root: ../main.tex -*-
%!TEX root = ../main.tex
% this file is called up by main.tex
% content in this file will be fed into the main document
% vim:nospell textwidth=180 foldlevelstart=3 foldlevel=3 conceallevel=0

\begin{table}[p]
    \centering
    \caption[Governing equations and boundary conditions of the \glsfmtshort{dfn} model]{Governing equations and boundary conditions of the \glsfmtlong{dfn} model}
    \label{tbl:dfneqns}
    \begingroup
    \makeatletter\def\f@size{9.8}\check@mathfonts
    \addtolength{\jot}{0.875em}
    \begin{tabular*}{\textwidth}{@{} l | l r l r @{}}
        \toprule
        \multicolumn{1}{c}{Region} & Governing equations & \multicolumn{2}{c}{Boundary conditions} & {} \\
        \midrule
    \multicolumn{1}{l |}{{\rotatebox[origin=c]{90}{\makecell{\footnotesize Separator\\ \scriptsize $\lambda \in \{\text{sep}\}$}}}} &
    % \multicolumn{3}{c}{\fbox{$ l_\text{neg} \coloneqq l_\text{n},\, l_\text{sep} \coloneqq l_\text{s},\, l_\text{pos} \coloneq l_\text{p}$}} &{} \\[0.5em]
    % {} &
    % $\begin{aligned}[t]
    %     \vphantom{\diffp{c_\text{e}}{x}{\mathrlap{x = l^{+}_\text{neg}}}} \varepsilon_\lambda \diffp{c_\text{e}}{t} &= \diffp{}{x}\left(D_\effmu \diffp{c_\text{e}}{x} \right) \\[-0.75em]
    % \end{aligned}$ &
    % $\begin{aligned}[t]
    % c_\text{e}\Bigr\rvert_{\mathrlap{x=l^{-}_\text{n}}}\hspace{5mm} &= c_\text{e}\Bigr\rvert_{\mathrlap{x=l^{+}_\text{n}}},\\[-0.75em]
    % c_\text{e}\Bigr\rvert_{\mathrlap{x=(l_{\text{n}} + l_\text{s})^{-}}}\hspace{5mm} &= c_\text{e}\Bigr\rvert_{\mathrlap{x=(l_{\text{n}} + l_\text{s})^{+}}},\\[1.25em]
    % \end{aligned}$ &
    % $\begin{aligned}[t]
    %     D_{\text{\tiny eff}_\text{n}}\!\! \! \!\, \diffp{c_\text{e}}{x}{\mathrlap{x = l^{-}_\text{n}}}\hspace{5mm} &=D_{\text{\tiny eff}_\text{s}}\!\!\!\!\,\diffp{c_\text{e}}{x}{\mathrlap{x = l^{+}_\text{n}}}\\[-0.75em]
    %     D_{\text{\tiny eff}_\text{s}}\!\! \! \!\, \diffp{c_\text{e}}{x}{\mathrlap{x=(l_{\text{n}} + l_\text{s})^{-}}}\hspace{5mm} &=D_{\text{\tiny eff}_\text{p}}\!\!\!\!\,\diffp{c_\text{e}}{x}{\mathrlap{x=(l_{\text{n}} + l_\text{s})^{+}}}\\[1.25em]
    % \end{aligned}$ &
    % $\begin{aligned}
    %     \refstepcounter{equation}(\theequation) \\[-0.75em]
    % \end{aligned}$
    % \\
    % {} &
    % $\begin{aligned}
    %     \frac{I}{A} &= \diffp{}{x}\left(\kappa_\effmu \diffp{\phi_\text{e}}{x}\right) + \diffp{}{x}\left(\kappa_\effmu \frac{2 R T(t)}{F} (t^0_{+}-1)\diffp{ \ln c_\text{e}}{x}\right) \\[-0.75em]
    % \end{aligned}$
    % & $\begin{aligned}[t]
    % \vphantom{\diffp{\phi_\text{e}}{x}{\mathrlap{x = l^{+}_\text{n}}}} \phi_\text{e}\Bigr\rvert_{\mathrlap{x=l^{-}_\text{n}}}\hspace{5mm} &= \phi_\text{e}\Bigr\rvert_{\mathrlap{x=l^{+}_\text{n}}},\\[-0.75em]
    % \phi_\text{e}\Bigr\rvert_{\mathrlap{x=(l_{\text{n}} + l_\text{s})^{-}}}\hspace{5mm} &= \phi_\text{e}\Bigr\rvert_{\mathrlap{x=(l_{\text{n}} + l_\text{s})^{-}}},\\
    % \end{aligned}$ &
    % $\begin{aligned}[t]
    %     \kappa_{\text{\tiny eff}_\text{n}}\!\! \! \!\, \diffp{c_\text{e}}{x}{\mathrlap{x = l^{-}_\text{n}}}\hspace{5mm} &=\kappa_{\text{\tiny eff}_\text{s}}\!\!\!\!\,\diffp{c_\text{e}}{x}{\mathrlap{x = l^{+}_\text{n}}}\\[-0.75em]
    %     \kappa_{\text{\tiny eff}_\text{s}}\!\! \! \!\, \diffp{c_\text{e}}{x}{\mathrlap{x=(l_{\text{n}} + l_\text{s})^{-}}}\hspace{5mm} &=\kappa_{\text{\tiny eff}_\text{p}}\!\!\!\!\,\diffp{c_\text{e}}{x}{\mathrlap{x=(l_{\text{n}} + l_\text{s})^{+}}}\\
    % \end{aligned}$ &
    % $\begin{aligned}
    %     \refstepcounter{equation}(\theequation) \\[-0.75em]
    % \end{aligned}$
    % \\
    \bottomrule
\end{tabular*}
\endgroup
\begin{minipage}{\textwidth}
    \bigskip
    \begin{flushleft}
        \raggedright
        \makeatletter\def\f@size{12}\check@mathfonts
        $ \text{\textbullet{} } c_\text{e}  \coloneqq c_\text{e}(x,t),\, \phi_\text{e} \coloneqq \phi_\text{e}(x,t) \quad \big\{\, x \in [0,l_\text{tot}],\, (x=0)\symbol{"2259} \text{\footnotesize neg/Cucc},\, (x=l_\text{tot})\symbol{"2259} \text{\footnotesize pos/Alcc}\, \big\}$
        \\[0.9em]
        {\raggedright \small \uline{\lambdainnegpos}}
        $\begin{alignedat}{2}
            & \text{\textbullet{} } c_\slambda & & \coloneqq c_\slambda(r,t),\, c_\slambdasurf \coloneqq c_\slambda(r=R_\plambda,t) \quad \big\{\, r \in [0,R_\plambda],\, (r=0)\symbol{"2259} \text{\footnotesize center},\, (r=R_\plambda)\symbol{"2259} \text{\footnotesize surface}\, \big\} \\[0.9em]
            % & \text{\textbullet{} } c_\slambdasurf & & \coloneqq c_\slambda(r=R_\plambda,t)\\
            & \text{\textbullet{} } \phi_\slambda & & \coloneqq \phi_\slambda(x_\lambda,t),\, j_\lambda \coloneqq j_\lambda(x_\lambda,t) \quad \big\{\, x_\lambda \subset x, \, x_\text{neg} \in [0,l_\text{pos}],\, x_\text{pos} \in [l_{\text{pos}+\text{neg}},l_\text{tot}]\, \big\} \\[0.9em]
            & \text{\textbullet{} } \eta_\lambda & & \coloneqq \eta_\lambda(x,t) = \phi_\slambda(x,t) - \phi_\text{e}(x,t) - \mathcal{U}_\lambda(c_\slambdasurf) \\
            & \text{\textbullet{} } \sigma_\efflambda & & = \sigma_\lambda \varepsilon_\slambda,\, D_\sefflambda = D_\slambda e^{\frac{-E_{\text{a},D_\slambda}}{R}\left(\frac{1}{T(t)} - \frac{1}{T_\text{sink}}\right)},\, k_\refflambda = k_\lambdar e^{\frac{-E_{\text{a},k_\lambdar}}{R}\left(\frac{1}{T(t)} - \frac{1}{T_\text{sink}}\right)} \\[0.9em]
        \end{alignedat}$
        {\raggedright \small \uline{\muinnegseppos}}\\[0.5ex]
        $\begin{alignedat}{2}
            & \text{\textbullet{} } D_\effmu & & = D \varepsilon_\lambda^{\text{brugg}_\lambda} \\
            & \text{\textbullet{} } D & & \coloneqq D(\scriptstyle{c_\text{e},T}\,\textstyle) = 10^{-4} \times 10^{-4.43 - \frac{54}{T(t) - 229 - 5\times10^{-3} c_\text{e}(x,t)} - 0.22\times10^{-3} c_\text{e}(x,t)} \\
        \end{alignedat}$
        \\
        \makeatletter\def\f@size{14}\check@mathfonts
        $\begin{alignedat}{2}
            & \text{\textbullet{} } \kappa_\effmu & & = \kappa \varepsilon_\lambda^{\text{brugg}_\lambda} \\
            & \text{\textbullet{} } \kappa & & \coloneqq \kappa\scriptstyle{(c_\text{e},T)}\; = \; \parbox[t]{11.60cm}{$\scriptstyle 10^{-4} \times c_\text{e}(x,t)\Big(-10.5 + 0.668\times10^{-3} c_\text{e}(x,t) + 0.494\times10^{-6} c_\text{e}^2(x,t) + \big(0.074 - 1.78\times10^{-5}c_\text{e}(x,t)$ \\ \hspace*{\fill} $\scriptstyle - 8.86\times10^{-10}c_\text{e}^2(x,t)\big)T(t) + \big(-6.96\times10^{-5} + 2.8\times10^{-8} c_\text{e}(x,t)\big)T^2(t)\Big)^2$}\\
        \end{alignedat}$
    \end{flushleft}
\end{minipage}
\end{table}

